Remove dependency of LowParse.Spec.Int.fsti on Endianness*

src/lowparse/LowParse.Spec.Int.Unique.fst
@@ -4,14 +4,17 @@ module Aux = LowParse.Spec.Int.Aux
 module I = LowParse.Spec.Int
 module Seq = FStar.Seq
 
+module U8 = FStar.UInt8
+module U16 = FStar.UInt16
+module U32 = FStar.UInt32
+
 open LowParse.Spec.Base
+
+friend LowParse.Spec.Int
 
 let le_refl (x y: int) : Lemma (requires (x <= y /\ y <= x)) (ensures (x == y)) = ()
 
-let parse_u8_unique
-  (b: bytes)
-: Lemma
-  (parse Aux.parse_u8 b == parse I.parse_u8 b)
+let parse_u8_unique b
 = if Seq.length b < 1
   then ()
   else begin
@@ -24,20 +27,12 @@ let parse_u8_unique
     ()
   end
 
-module U8 = FStar.UInt8
-
-let serialize_u8_unique
-  (x: U8.t)
-: Lemma
-  (serialize Aux.serialize_u8 x == serialize I.serialize_u8 x)
+let serialize_u8_unique x
 = Classical.forall_intro parse_u8_unique;
   let s : serializer I.parse_u8 = serialize_ext Aux.parse_u8 Aux.serialize_u8 I.parse_u8 in
   serializer_unique I.parse_u8 I.serialize_u8 s x
 
-let parse_u16_unique
-  (b: bytes)
-: Lemma
-  (parse Aux.parse_u16 b == parse I.parse_u16 b)
+let parse_u16_unique b
 = if Seq.length b < 2
   then ()
   else begin
@@ -50,20 +45,12 @@ let parse_u16_unique
     ()
   end
 
-module U16 = FStar.UInt16
-
-let serialize_u16_unique
-  (x: U16.t)
-: Lemma
-  (serialize #_ #_ #Aux.parse_u16 Aux.serialize_u16 x == serialize I.serialize_u16 x)
+let serialize_u16_unique x
 = Classical.forall_intro parse_u16_unique;
   let s : serializer I.parse_u16 = serialize_ext Aux.parse_u16 Aux.serialize_u16 I.parse_u16 in
   serializer_unique I.parse_u16 I.serialize_u16 s x
 
-let parse_u32_unique
-  (b: bytes)
-: Lemma
-  (parse Aux.parse_u32 b == parse I.parse_u32 b)
+let parse_u32_unique b
 = if Seq.length b < 4
   then ()
   else begin
@@ -76,12 +63,7 @@ let parse_u32_unique
     ()
   end
 
-module U32 = FStar.UInt32
-
-let serialize_u32_unique
-  (x: U32.t)
-: Lemma
-  (serialize #_ #_ #Aux.parse_u32 Aux.serialize_u32 x == serialize I.serialize_u32 x)
+let serialize_u32_unique x
 = Classical.forall_intro parse_u32_unique;
   let s : serializer I.parse_u32 = serialize_ext Aux.parse_u32 Aux.serialize_u32 I.parse_u32 in
   serializer_unique I.parse_u32 I.serialize_u32 s x
