src/lowparse/LowParse.SLow.Int.fst
@@ -8,6 +8,8 @@ module U16 = FStar.UInt16
 module U32 = FStar.UInt32
 module B32 = FStar.Bytes
 
+friend LowParse.Spec.Int
+
 let parse32_u8 =
   (fun input ->
     [@inline_let]
