src/lowparse/LowParse.Spec.Int.Unique.fsti
@@ -1,0 +1,41 @@
+module LowParse.Spec.Int.Unique
+
+module Aux = LowParse.Spec.Int.Aux
+module I = LowParse.Spec.Int
+module Seq = FStar.Seq
+
+module U8 = FStar.UInt8
+module U16 = FStar.UInt16
+module U32 = FStar.UInt32
+
+open LowParse.Spec.Base
+
+val parse_u8_unique
+  (b: bytes)
+: Lemma
+  (parse Aux.parse_u8 b == parse I.parse_u8 b)
+
+val serialize_u8_unique
+  (x: U8.t)
+: Lemma
+  (serialize Aux.serialize_u8 x == serialize I.serialize_u8 x)
+
+val parse_u16_unique
+  (b: bytes)
+: Lemma
+  (parse Aux.parse_u16 b == parse I.parse_u16 b)
+
+val serialize_u16_unique
+  (x: U16.t)
+: Lemma
+  (serialize #_ #_ #Aux.parse_u16 Aux.serialize_u16 x == serialize I.serialize_u16 x)
+
+val parse_u32_unique
+  (b: bytes)
+: Lemma
+  (parse Aux.parse_u32 b == parse I.parse_u32 b)
+
+val serialize_u32_unique
+  (x: U32.t)
+: Lemma
+  (serialize #_ #_ #Aux.parse_u32 Aux.serialize_u32 x == serialize I.serialize_u32 x)
