src/lowparse/LowParse.Spec.Int.fst
@@ -9,17 +9,50 @@ module U32 = FStar.UInt32
 
 let parse_u8 = Aux.parse_u8
 
+val parse_u8_spec
+  (b: bytes)
+: Lemma
+  (requires (Seq.length b >= 1))
+  (ensures (
+    let pp = parse parse_u8 b in
+    Some? pp /\ (
+    let (Some (v, consumed)) = pp in
+    U8.v v == E.be_to_n (Seq.slice b 0 1)
+  )))
+
 let parse_u8_spec b = Aux.parse_u8_spec b
 
 let serialize_u8 = Aux.serialize_u8
 
 let parse_u16 = Aux.parse_u16
 
+val parse_u16_spec
+  (b: bytes)
+: Lemma
+  (requires (Seq.length b >= 2))
+  (ensures (
+    let pp = parse parse_u16 b in
+    Some? pp /\ (
+    let (Some (v, consumed)) = pp in
+    U16.v v == E.be_to_n (Seq.slice b 0 2)
+  )))
+
 let parse_u16_spec b = Aux.parse_u16_spec b
 
 let serialize_u16 = Aux.serialize_u16
 
 let parse_u32 = Aux.parse_u32
+
+val parse_u32_spec
+  (b: bytes)
+: Lemma
+  (requires (Seq.length b >= 4))
+  (ensures (
+    let pp = parse parse_u32 b in
+    Some? pp /\ (
+    let (Some (v, consumed)) = pp in
+    U32.v v == E.be_to_n (Seq.slice b 0 4)
+  )))
 
 let parse_u32_spec = Aux.parse_u32_spec
 
